cleaned up theorem 2 proof

thm2_TEMP.thy
@@ -41,7 +41,7 @@ definition D :: "real" where "D = 0.6"
 (*If they appear free here, they are for any input, this is a statement about
 this input, not for all input, *)
 theorem conf_vcs:
-  fixes x_1 x_2 y_2 :: real
+  fixes x_1 x_2 y_1 :: real
 assumes "\<epsilon> \<ge> 0" and 
   "(y_1 = (P * x_1) + (D * x_2)) \<longrightarrow>
              \<bar>(denormO 1 (annout 2 1 [(normI 1 x_1), (normI 2 x_2)]) ) - y_1 \<bar> \<le> \<epsilon>"
@@ -49,46 +49,22 @@ shows "(conf_sin \<epsilon> angleOutputE AnglePIDANN AnglePID_C)"
   sorry
 
 
-(*Preliminary, monotonicity of the f function. *)
+(*This is a shorthand for the specification function for our example, 
+with the denormilisation applied, to help with reasoning.  *)
 
-definition spec_f :: "real \<Rightarrow> real \<Rightarrow> real" where
-"spec_f x_1 x_2 = (P * x_1) + (D * x_2)"
-
-definition norm_spec_f :: "real \<Rightarrow> real \<Rightarrow> real" where 
-"norm_spec_f x_1 x_2 = (denormI 1 (x_1 * P) + (denormI 2 (x_2 * D) ))"
-
-definition norm_spec_f_2 :: "real \<Rightarrow> real \<Rightarrow> real" where 
-"norm_spec_f_2 x_1 x_2 = 
+definition norm_spec :: "real \<Rightarrow> real \<Rightarrow> real" where 
+"norm_spec x_1 x_2 = 
   (P * denormI 1 (x_1) + (D * denormI 2 (x_2)) )"
 
-lemma norm_spec_f_mono: 
+lemma norm_spec_mono: 
   fixes x_1 :: real and x_2 :: real and y_1 :: real and y_2 :: real
   assumes "P > 0" and "D > 0" and 
     "(snd(inRanges(1)) > fst(inRanges(1)) \<and> snd(inRanges(2)) > fst(inRanges(2)) \<and> snd(annRange) > fst(annRange))"
-  shows "x_1 \<le> y_1 \<and> x_2 \<le> y_2 \<longrightarrow> (norm_spec_f x_1 x_2) \<le> (norm_spec_f y_1 y_2)"
-  using assms apply (simp add: mono_denormI mono_norm norm_spec_f_def ordered_ab_semigroup_add_class.add_mono)
-  by (smt (verit, best) One_nat_def assms(3) mono_denormI mult.commute mult_left_mono)
- 
-
-lemma norm_spec_f_2_mono: 
-  fixes x_1 :: real and x_2 :: real and y_1 :: real and y_2 :: real
-  assumes "P > 0" and "D > 0" and 
-    "(snd(inRanges(1)) > fst(inRanges(1)) \<and> snd(inRanges(2)) > fst(inRanges(2)) \<and> snd(annRange) > fst(annRange))"
-  shows "x_1 \<le> y_1 \<and> x_2 \<le> y_2 \<longrightarrow> (norm_spec_f_2 x_1 x_2) \<le> (norm_spec_f_2 y_1 y_2)"
-  using assms apply (simp add: mono_denormI mono_norm norm_spec_f_def mono_normI
+  shows "x_1 \<le> y_1 \<and> x_2 \<le> y_2 \<longrightarrow> (norm_spec x_1 x_2) \<le> (norm_spec y_1 y_2)"
+  using assms apply (simp add: mono_denormI mono_norm norm_spec_def mono_normI
             ordered_ab_semigroup_add_class.add_mono)
-  by (smt (verit, best) assms(3) mono_denormI mono_normI mult.commute mult_le_cancel_left_pos norm_spec_f_2_def)
+  by (smt (verit, ccfv_SIG) One_nat_def assms(3) mono_denormI mult_left_mono)
   
-
-lemma spec_f_mono: 
-  fixes x_1 :: real and x_2 :: real and y_1 :: real and y_2 :: real
-  assumes "P > 0" and "D > 0"
-  shows "x_1 \<le> y_1 \<and> x_2 \<le> y_2 \<longrightarrow> (spec_f x_1 x_2) \<le> (spec_f y_1 y_2)"
-  by (simp add: assms(1) assms(2) ordered_ab_semigroup_add_class.add_mono spec_f_def)
-
-term "[ ((normI 1 (inRanges(1).1)), ((normI 1 (inRanges(1).2)))), 
-         ((normI 2 (inRanges(2).1)), ((normI 2 (inRanges(2).2)))) ]"
-
 (*Interval definition: *)
 definition int :: "(real \<times> real) list" where
 "int = [ ((normI 1 (inRanges(1).1)), ((normI 1 (inRanges(1).2)))), 
@@ -105,7 +81,8 @@ term "snd(int(2))"
 (*Abbreviation for readability, referring to the f_ann as annout 2 1 to correspond 
 to the last layer of our example: *)
 abbreviation "f_ann x y \<equiv> annout 2 1 [x,y]"
-    
+
+term "f_ann 0 0"
 
 lemma spec_mono_ann:
   fixes x_1 x_2 y_1 y_2 :: real and
@@ -193,9 +170,13 @@ we already have int, meaningless without the splits.
 
 We need it to be automatic, automated evaluation as well. 
 
+Apply eval, eval doesn't pause halfway through, solves goal through 
+evaluation, we don't want this. evaluating, partial evaluation ? 
 *)
 
-lemma marabou_evaluated_results: 
+
+
+lemma marabou_combined_results: 
   fixes x1 x2 :: real
   assumes "x1 \<ge> fst(int(1)) \<and> 
           x1 \<le> snd(int(1)) \<and>
@@ -213,6 +194,7 @@ proof -
           x2 \<le> 1 \<longrightarrow> 
           \<not> f_ann x1 x2 \<ge> (1 / 3900)
           " sorry
+      
   have 2: "x1 \<ge> 0 \<and> 
           x1 \<le> 1 \<and>
           x2 \<ge> 0 \<and>
@@ -225,37 +207,6 @@ proof -
 denormI_def normO_def outRanges_def \<epsilon>_def
     apply (simp)
     done    
-qed
-
-
-
-
-
-lemma marabou_combined_results: 
-  fixes x1 x2 :: real
-  assumes "x1 \<ge> fst(int(1)) \<and> 
-          x1 \<le> snd(int(1)) \<and>
-          x2 \<ge> fst(int(2)) \<and>
-          x2 \<le> snd(int(2))"
-  shows "
-          \<not> f_ann x1 x2 \<ge> normO 1 ((P * denormI 1 (fst(int(1))) + (D * denormI 2 (fst(int(2)))) ) + \<epsilon>)
-           \<and>           
-          \<not> f_ann x1 x2 \<le> normO 1 ((P * denormI 1 (snd(int(1))) + (D * denormI 2 (snd(int(2)))) ) - \<epsilon>)
-" 
-proof - 
-  have 1: "x1 \<ge> normI 1 (inRanges(1).1) \<and> 
-          x1 \<le> normI 1 (inRanges(1).2) \<and>
-          x2 \<ge> normI 2 (inRanges(2).1) \<and>   
-          x2 \<le> normI 2 (inRanges(2).2) \<longrightarrow> 
-          \<not> f_ann x1 x2 \<ge> normO 1 ((P * denormI 1 (fst(int(1))) + (D * denormI 2 (fst(int(2)))) ) + \<epsilon>)
-          " sorry
-  have 2: "x1 \<ge> normI 1 (inRanges(1).1) \<and> 
-          x1 \<le> normI 1 (inRanges(1).2) \<and>
-          x2 \<ge> normI 2 (inRanges(2).1) \<and>
-          x2 \<le> normI 2 (inRanges(2).2) \<longrightarrow>
-          \<not> f_ann x1 x2 \<le> normO 1 ((P * denormI 1 (snd(int(1))) + (D * denormI 2 (snd(int(2)))) ) - \<epsilon>)
-        " sorry
-  from 1 2 show "?thesis" using assms by (simp add: int_def) 
 qed
 
 
@@ -281,20 +232,11 @@ theorem controller_conformance:
   
   (*We need to show our goal under a range of our bound input variables. 
     This has to be here, the range assumptions, not as an assumption. *)
-  shows " (conf_sin \<epsilon> angleOutputE AnglePIDANN AnglePID_C)" 
-   apply (rule conf_vcs)  
-  (*Discharge first assumption: *)
-   apply (simp add: assms(1))
+shows " (conf_sin \<epsilon> angleOutputE AnglePIDANN AnglePID_C)"
 
 proof - 
-  (*Assumption, if we take the ranges of *)
-  have 1:"x_1 \<ge> inRanges(1).1 \<and> 
-          x_1 \<le> inRanges(1).2 \<and>
-          x_2 \<ge> inRanges(2).1 \<and>
-          x_2 \<le> inRanges(2).2" using assms by simp
-    (*This works: *)
-   
-  from marabou_evaluated_results[where ?x1.0="normI 1 x_1" and ?x2.0="normI 2 x_2"] have m3: 
+
+  from marabou_combined_results[where ?x1.0="normI 1 x_1" and ?x2.0="normI 2 x_2"] have m3: 
           "normI 1 x_1 \<ge> normI 1 (inRanges(1).1) \<and> 
           normI 1 x_1 \<le> normI 1 (inRanges(1).2) \<and>
           normI 2 x_2 \<ge> normI 2 (inRanges(2).1) \<and>
@@ -308,51 +250,28 @@ proof -
            \<and>
           \<not> annout 2 1 [normI 1 x_1, normI 2 x_2] \<le> normO 1 ((P * denormI 1 (snd(int(1))) + (D * denormI 2 (snd(int(2)))) ) - \<epsilon>)"
     by (simp add: int_def)
-    
-  have "... \<longrightarrow>
-  
-          normI 1 x_1 \<ge> normI 1 (inRanges(1).1) \<and> 
-          normI 1 x_1 \<le> normI 1 (inRanges(1).2) \<and>
-          normI 2 x_2 \<ge> normI 2 (inRanges(2).1) \<and>
-          normI 2 x_2 \<le> normI 2 (inRanges(2).2) \<and>
-   annout 2 1 [normI 1 x_1, normI 2 x_2] \<le> normO 1 ((P * denormI 1 (fst(int(1))) + (D * denormI 2 (fst(int(2)))) ) + \<epsilon>)
-     \<and>
-    annout 2 1 [normI 1 x_1, normI 2 x_2] \<ge> normO 1 ((P * denormI 1 (snd(int(1))) + (D * denormI 2 (snd(int(2)))) ) - \<epsilon>)"
-     using nle_le by blast
-     
 
-   have "... \<longrightarrow> 
-          normI 1 x_1 \<ge> normI 1 (inRanges(1).1) \<and> 
-          normI 1 x_1 \<le> normI 1 (inRanges(1).2) \<and>
-          normI 2 x_2 \<ge> normI 2 (inRanges(2).1) \<and>
-          normI 2 x_2 \<le> normI 2 (inRanges(2).2) \<and>
-     annout 2 1 [normI 1 x_1, normI 2 x_2] \<le> normO 1 (norm_spec_f_2 (fst(int(1))) (fst(int(2))) + \<epsilon>)
-     \<and> 
-     annout 2 1 [normI 1 x_1, normI 2 x_2] \<ge> normO 1 (norm_spec_f_2 (snd(int(1))) (snd(int(2))) - \<epsilon>)
-    "
-     unfolding norm_spec_f_2_def
-     apply (simp)
-     done
-
-   have "... \<longrightarrow> 
+   have "... = (
     
           normI 1 x_1 \<ge> normI 1 (inRanges(1).1) \<and> 
           normI 1 x_1 \<le> normI 1 (inRanges(1).2) \<and>
           normI 2 x_2 \<ge> normI 2 (inRanges(2).1) \<and>
           normI 2 x_2 \<le> normI 2 (inRanges(2).2) \<and>
-     annout 2 1 [normI 1 x_1, normI 2 x_2] \<ge> normO 1 (norm_spec_f_2 (snd(int(1))) (snd(int(2))) - \<epsilon>)
+     annout 2 1 [normI 1 x_1, normI 2 x_2] \<ge> normO 1 (norm_spec (snd(int(1))) (snd(int(2))) - \<epsilon>)
       \<and> 
-     annout 2 1 [normI 1 x_1, normI 2 x_2] \<le> normO 1 (norm_spec_f_2 (fst(int(1))) (fst(int(2))) + \<epsilon>)
-    "
+     annout 2 1 [normI 1 x_1, normI 2 x_2] \<le> normO 1 (norm_spec (fst(int(1))) (fst(int(2))) + \<epsilon>)
+    )"
+     using nle_le
+     unfolding norm_spec_def
      apply (simp)
-     done
+     using m3 by force
   
   (*Important step, get from the intervals to the actual fixed variables:
     We can still have this, at the moment, be on the normalised ranges.  *)
-   have "... \<longrightarrow> 
-     annout 2 1 [normI 1 x_1, normI 2 x_2] \<ge> normO 1 (norm_spec_f_2 (normI 1 x_1) (normI 2 x_2) - \<epsilon>)
+   have "... \<longrightarrow>
+     annout 2 1 [normI 1 x_1, normI 2 x_2] \<ge> normO 1 (norm_spec (normI 1 x_1) (normI 2 x_2) - \<epsilon>)
      \<and> 
-     annout 2 1 [normI 1 x_1, normI 2 x_2] \<le> normO 1 (norm_spec_f_2 (normI 1 x_1) (normI 2 x_2) + \<epsilon>)
+     annout 2 1 [normI 1 x_1, normI 2 x_2] \<le> normO 1 (norm_spec (normI 1 x_1) (normI 2 x_2) + \<epsilon>)
     "
      apply (rule impI)
      apply (rule spec_mono_ann[where f="f_ann"])
@@ -361,83 +280,78 @@ proof -
           normI 1 x_1 \<le> normI 1 (inRanges(1).2) \<and>
           normI 2 x_2 \<ge> normI 2 (inRanges(2).1) \<and>
           normI 2 x_2 \<le> normI 2 (inRanges(2).2) \<and>
-          annout 2 1 [normI 1 x_1, normI 2 x_2] \<ge> normO 1 (norm_spec_f_2 (snd(int(1))) (snd(int(2))) - \<epsilon>)
+          annout 2 1 [normI 1 x_1, normI 2 x_2] \<ge> normO 1 (norm_spec (snd(int(1))) (snd(int(2))) - \<epsilon>)
       \<and> 
-     annout 2 1 [normI 1 x_1, normI 2 x_2] \<le> normO 1 (norm_spec_f_2 (fst(int(1))) (fst(int(2))) + \<epsilon>)"
-     show "\<forall> x_1 x_2 y_1 y_2. x_1 \<le> y_1 \<and> x_2 \<le> y_2 \<longrightarrow> norm_spec_f_2 x_1 x_2 \<le> norm_spec_f_2 y_1 y_2" 
-       using assms apply (simp add: norm_spec_f_2_mono)
+     annout 2 1 [normI 1 x_1, normI 2 x_2] \<le> normO 1 (norm_spec (fst(int(1))) (fst(int(2))) + \<epsilon>)"
+     show "\<forall> x_1 x_2 y_1 y_2. x_1 \<le> y_1 \<and> x_2 \<le> y_2 \<longrightarrow> norm_spec x_1 x_2 \<le> norm_spec y_1 y_2" 
+       using assms apply (simp add: norm_spec_mono)
        done
 
      show "fst (int(1)) \<le> normI 1 x_1 \<and> normI 1 x_1 \<le> snd (int(1))"
-       by (metis \<open>normI 1 (fst (inRanges(1)\<^sub>s)) \<le> normI 1 x_1 \<and> normI 1 x_1 \<le> normI 1 (snd (inRanges(1)\<^sub>s)) \<and> normI 2 (fst (inRanges(2)\<^sub>s)) \<le> normI 2 x_2 \<and> normI 2 x_2 \<le> normI 2 (snd (inRanges(2)\<^sub>s)) \<and> normO 1 (norm_spec_f_2 (snd (thm2_TEMP.int(1)\<^sub>s)) (snd (thm2_TEMP.int(2)\<^sub>s)) - \<epsilon>) \<le> f_ann (normI 1 x_1) (normI 2 x_2) \<and> f_ann (normI 1 x_1) (normI 2 x_2) \<le> normO 1 (norm_spec_f_2 (fst (thm2_TEMP.int(1)\<^sub>s)) (fst (thm2_TEMP.int(2)\<^sub>s)) + \<epsilon>)\<close> cancel_comm_monoid_add_class.diff_cancel fst_conv nth_Cons_0 snd_conv thm2_TEMP.int_def)
+       by (metis \<open>normI 1 (fst (inRanges(1)\<^sub>s)) \<le> normI 1 x_1 \<and> normI 1 x_1 \<le> normI 1 (snd (inRanges(1)\<^sub>s)) \<and> normI 2 (fst (inRanges(2)\<^sub>s)) \<le> normI 2 x_2 \<and> normI 2 x_2 \<le> normI 2 (snd (inRanges(2)\<^sub>s)) \<and> normO 1 (norm_spec (snd (thm2_TEMP.int(1)\<^sub>s)) (snd (thm2_TEMP.int(2)\<^sub>s)) - \<epsilon>) \<le> f_ann (normI 1 x_1) (normI 2 x_2) \<and> f_ann (normI 1 x_1) (normI 2 x_2) \<le> normO 1 (norm_spec (fst (thm2_TEMP.int(1)\<^sub>s)) (fst (thm2_TEMP.int(2)\<^sub>s)) + \<epsilon>)\<close> cancel_comm_monoid_add_class.diff_cancel fst_conv nth_Cons_0 snd_conv thm2_TEMP.int_def)
        
 
      show "fst (int(2)\<^sub>s) \<le> normI 2 x_2  \<and> normI 2 x_2 \<le> snd (int(2)\<^sub>s)"
-       by (metis One_nat_def \<open>normI 1 (fst (inRanges(1)\<^sub>s)) \<le> normI 1 x_1 \<and> normI 1 x_1 \<le> normI 1 (snd (inRanges(1)\<^sub>s)) \<and> normI 2 (fst (inRanges(2)\<^sub>s)) \<le> normI 2 x_2 \<and> normI 2 x_2 \<le> normI 2 (snd (inRanges(2)\<^sub>s)) \<and> normO 1 (norm_spec_f_2 (snd (thm2_TEMP.int(1)\<^sub>s)) (snd (thm2_TEMP.int(2)\<^sub>s)) - \<epsilon>) \<le> f_ann (normI 1 x_1) (normI 2 x_2) \<and> f_ann (normI 1 x_1) (normI 2 x_2) \<le> normO 1 (norm_spec_f_2 (fst (thm2_TEMP.int(1)\<^sub>s)) (fst (thm2_TEMP.int(2)\<^sub>s)) + \<epsilon>)\<close> diff_Suc_1 nat_1_add_1 nth_Cons_0 nth_Cons_Suc plus_1_eq_Suc split_pairs thm2_TEMP.int_def)
+       by (metis One_nat_def \<open>normI 1 (fst (inRanges(1)\<^sub>s)) \<le> normI 1 x_1 \<and> normI 1 x_1 \<le> normI 1 (snd (inRanges(1)\<^sub>s)) \<and> normI 2 (fst (inRanges(2)\<^sub>s)) \<le> normI 2 x_2 \<and> normI 2 x_2 \<le> normI 2 (snd (inRanges(2)\<^sub>s)) \<and> normO 1 (norm_spec (snd (thm2_TEMP.int(1)\<^sub>s)) (snd (thm2_TEMP.int(2)\<^sub>s)) - \<epsilon>) \<le> f_ann (normI 1 x_1) (normI 2 x_2) \<and> f_ann (normI 1 x_1) (normI 2 x_2) \<le> normO 1 (norm_spec (fst (thm2_TEMP.int(1)\<^sub>s)) (fst (thm2_TEMP.int(2)\<^sub>s)) + \<epsilon>)\<close> diff_Suc_1 nat_1_add_1 nth_Cons_0 nth_Cons_Suc plus_1_eq_Suc split_pairs thm2_TEMP.int_def)
        
 
-    show "0 \<le> \<epsilon>" 
+     show "0 \<le> \<epsilon>" 
        using assms by simp
 
      show "fst (outRanges ! 0) < snd (outRanges ! 0) \<and> fst annRange < snd annRange" using assms by simp
         
-
      show 
-     "f_ann (normI 1 x_1) (normI 2 x_2) \<le> normO 1 (norm_spec_f_2 (fst (int(1))) (fst (int(2))) + \<epsilon>) \<and>
-      f_ann (normI 1 x_1) (normI 2 x_2) \<ge> normO 1 (norm_spec_f_2 (snd (int(1))) (snd (thm2_TEMP.int(2))) - \<epsilon>)"
-       using \<open>normI 1 (fst (inRanges(1)\<^sub>s)) \<le> normI 1 x_1 \<and> normI 1 x_1 \<le> normI 1 (snd (inRanges(1)\<^sub>s)) \<and> normI 2 (fst (inRanges(2)\<^sub>s)) \<le> normI 2 x_2 \<and> normI 2 x_2 \<le> normI 2 (snd (inRanges(2)\<^sub>s)) \<and> normO 1 (norm_spec_f_2 (snd (thm2_TEMP.int(1)\<^sub>s)) (snd (thm2_TEMP.int(2)\<^sub>s)) - \<epsilon>) \<le> f_ann (normI 1 x_1) (normI 2 x_2) \<and> f_ann (normI 1 x_1) (normI 2 x_2) \<le> normO 1 (norm_spec_f_2 (fst (thm2_TEMP.int(1)\<^sub>s)) (fst (thm2_TEMP.int(2)\<^sub>s)) + \<epsilon>)\<close> by fastforce
+     "f_ann (normI 1 x_1) (normI 2 x_2) \<le> normO 1 (norm_spec (fst (int(1))) (fst (int(2))) + \<epsilon>) \<and>
+      f_ann (normI 1 x_1) (normI 2 x_2) \<ge> normO 1 (norm_spec (snd (int(1))) (snd (thm2_TEMP.int(2))) - \<epsilon>)"
+       using \<open>normI 1 (fst (inRanges(1)\<^sub>s)) \<le> normI 1 x_1 \<and> normI 1 x_1 \<le> normI 1 (snd (inRanges(1)\<^sub>s)) \<and> normI 2 (fst (inRanges(2)\<^sub>s)) \<le> normI 2 x_2 \<and> normI 2 x_2 \<le> normI 2 (snd (inRanges(2)\<^sub>s)) \<and> normO 1 (norm_spec (snd (thm2_TEMP.int(1)\<^sub>s)) (snd (thm2_TEMP.int(2)\<^sub>s)) - \<epsilon>) \<le> f_ann (normI 1 x_1) (normI 2 x_2) \<and> f_ann (normI 1 x_1) (normI 2 x_2) \<le> normO 1 (norm_spec (fst (thm2_TEMP.int(1)\<^sub>s)) (fst (thm2_TEMP.int(2)\<^sub>s)) + \<epsilon>)\<close> by fastforce
        
      qed
 
-     have "... \<longrightarrow> 
+     have "... = ( 
       f_ann (normI 1 x_1) (normI 2 x_2) \<ge> normO 1 (P * denormI 1 (normI 1 x_1) + D * denormI 2 (normI 2 x_2) - \<epsilon>) \<and>
-      f_ann (normI 1 x_1) (normI 2 x_2) \<le> normO 1 (P * denormI 1 (normI 1 x_1) + D * denormI 2 (normI 2 x_2) + \<epsilon>)"
-       unfolding norm_spec_f_2_def by simp
+      f_ann (normI 1 x_1) (normI 2 x_2) \<le> normO 1 (P * denormI 1 (normI 1 x_1) + D * denormI 2 (normI 2 x_2) + \<epsilon>))"
+       unfolding norm_spec_def by simp
     
-     have "... \<longrightarrow> 
+     have "... = ( 
       denormO 1 (f_ann (normI 1 x_1) (normI 2 x_2)) \<ge> denormO 1 (normO 1 (P * denormI 1 (normI 1 x_1) + D * denormI 2 (normI 2 x_2) - \<epsilon>)) \<and>
-      denormO 1 (f_ann (normI 1 x_1) (normI 2 x_2)) \<le> denormO 1 (normO 1 (P * denormI 1 (normI 1 x_1) + D * denormI 2 (normI 2 x_2) + \<epsilon>))"
+      denormO 1 (f_ann (normI 1 x_1) (normI 2 x_2)) \<le> denormO 1 (normO 1 (P * denormI 1 (normI 1 x_1) + D * denormI 2 (normI 2 x_2) + \<epsilon>)))"
        using assms apply (simp add: mono_denormO)
-       by (metis mono_denormO order_le_less)
+       by (smt (verit, ccfv_threshold) mono_denormO)
 
-     have "... \<longrightarrow> 
+     have "... = (
         denormO 1 (f_ann (normI 1 x_1) (normI 2 x_2)) \<ge> (P * denormI 1 (normI 1 x_1) + D * denormI 2 (normI 2 x_2) - \<epsilon>) \<and>
         denormO 1 (f_ann (normI 1 x_1) (normI 2 x_2)) \<le> (P * denormI 1 (normI 1 x_1) + D * denormI 2 (normI 2 x_2) + \<epsilon>)
-        "
+        )"
        using assms(2) output_norm_2 by presburger 
 
-      have "... \<longrightarrow> 
+      have "... = ( 
         denormO 1 (f_ann (normI 1 x_1) (normI 2 x_2)) \<ge> (P * x_1 + D * x_2 - \<epsilon>) \<and>
         denormO 1 (f_ann (normI 1 x_1) (normI 2 x_2)) \<le> (P * x_1 + D * x_2 + \<epsilon>)
-        "
+        )"
         using assms(2) input_norm2 by presburger
 
-    have "... \<longrightarrow> 
+    have "... = ( 
         \<bar>denormO 1 (f_ann (normI 1 x_1) (normI 2 x_2)) - (P * x_1 + D * x_2)\<bar> \<le> \<epsilon>
-        "
+        )"
       by linarith
 
-    have goal:"... \<longrightarrow> 
+    have goal:"... \<longrightarrow> ( 
           y_1 = P * x_1 + D * x_2 \<longrightarrow> \<bar>denormO 1 (f_ann (normI 1 x_1) (normI 2 x_2)) - y_1\<bar> \<le> \<epsilon>
-        " by simp
+        )" apply simp
+        
+      done
 
-    have goal2:"normI 1 x_1 \<ge> normI 1 (inRanges(1).1) \<and> 
-          normI 1 x_1 \<le> normI 1 (inRanges(1).2) \<and>
-          normI 2 x_2 \<ge> normI 2 (inRanges(2).1) \<and>
-          normI 2 x_2 \<le> normI 2 (inRanges(2).2) \<longrightarrow> y_1 = P * x_1 + D * x_2 \<longrightarrow> \<bar>denormO 1 (f_ann (normI 1 x_1) (normI 2 x_2)) - y_1\<bar> \<le> \<epsilon>
-        "
-      using \<open>P * denormI 1 (normI 1 x_1) + D * denormI 2 (normI 2 x_2) - \<epsilon> \<le> denormO 1 (f_ann (normI 1 x_1) (normI 2 x_2)) \<and> denormO 1 (f_ann (normI 1 x_1) (normI 2 x_2)) \<le> P * denormI 1 (normI 1 x_1) + D * denormI 2 (normI 2 x_2) + \<epsilon> \<longrightarrow> P * x_1 + D * x_2 - \<epsilon> \<le> denormO 1 (f_ann (normI 1 x_1) (normI 2 x_2)) \<and> denormO 1 (f_ann (normI 1 x_1) (normI 2 x_2)) \<le> P * x_1 + D * x_2 + \<epsilon>\<close> \<open>denormO 1 (normO 1 (P * denormI 1 (normI 1 x_1) + D * denormI 2 (normI 2 x_2) - \<epsilon>)) \<le> denormO 1 (f_ann (normI 1 x_1) (normI 2 x_2)) \<and> denormO 1 (f_ann (normI 1 x_1) (normI 2 x_2)) \<le> denormO 1 (normO 1 (P * denormI 1 (normI 1 x_1) + D * denormI 2 (normI 2 x_2) + \<epsilon>)) \<longrightarrow> P * denormI 1 (normI 1 x_1) + D * denormI 2 (normI 2 x_2) - \<epsilon> \<le> denormO 1 (f_ann (normI 1 x_1) (normI 2 x_2)) \<and> denormO 1 (f_ann (normI 1 x_1) (normI 2 x_2)) \<le> P * denormI 1 (normI 1 x_1) + D * denormI 2 (normI 2 x_2) + \<epsilon>\<close> \<open>normI 1 (fst (inRanges(1)\<^sub>s)) \<le> normI 1 x_1 \<and> normI 1 x_1 \<le> normI 1 (snd (inRanges(1)\<^sub>s)) \<and> normI 2 (fst (inRanges(2)\<^sub>s)) \<le> normI 2 x_2 \<and> normI 2 x_2 \<le> normI 2 (snd (inRanges(2)\<^sub>s)) \<and> f_ann (normI 1 x_1) (normI 2 x_2) \<le> normO 1 (P * denormI 1 (fst (thm2_TEMP.int(1)\<^sub>s)) + D * denormI 2 (fst (thm2_TEMP.int(2)\<^sub>s)) + \<epsilon>) \<and> normO 1 (P * denormI 1 (snd (thm2_TEMP.int(1)\<^sub>s)) + D * denormI 2 (snd (thm2_TEMP.int(2)\<^sub>s)) - \<epsilon>) \<le> f_ann (normI 1 x_1) (normI 2 x_2) \<longrightarrow> normI 1 (fst (inRanges(1)\<^sub>s)) \<le> normI 1 x_1 \<and> normI 1 x_1 \<le> normI 1 (snd (inRanges(1)\<^sub>s)) \<and> normI 2 (fst (inRanges(2)\<^sub>s)) \<le> normI 2 x_2 \<and> normI 2 x_2 \<le> normI 2 (snd (inRanges(2)\<^sub>s)) \<and> f_ann (normI 1 x_1) (normI 2 x_2) \<le> normO 1 (norm_spec_f_2 (fst (thm2_TEMP.int(1)\<^sub>s)) (fst (thm2_TEMP.int(2)\<^sub>s)) + \<epsilon>) \<and> normO 1 (norm_spec_f_2 (snd (thm2_TEMP.int(1)\<^sub>s)) (snd (thm2_TEMP.int(2)\<^sub>s)) - \<epsilon>) \<le> f_ann (normI 1 x_1) (normI 2 x_2)\<close> \<open>normI 1 (fst (inRanges(1)\<^sub>s)) \<le> normI 1 x_1 \<and> normI 1 x_1 \<le> normI 1 (snd (inRanges(1)\<^sub>s)) \<and> normI 2 (fst (inRanges(2)\<^sub>s)) \<le> normI 2 x_2 \<and> normI 2 x_2 \<le> normI 2 (snd (inRanges(2)\<^sub>s)) \<and> normO 1 (norm_spec_f_2 (snd (thm2_TEMP.int(1)\<^sub>s)) (snd (thm2_TEMP.int(2)\<^sub>s)) - \<epsilon>) \<le> f_ann (normI 1 x_1) (normI 2 x_2) \<and> f_ann (normI 1 x_1) (normI 2 x_2) \<le> normO 1 (norm_spec_f_2 (fst (thm2_TEMP.int(1)\<^sub>s)) (fst (thm2_TEMP.int(2)\<^sub>s)) + \<epsilon>) \<longrightarrow> normO 1 (norm_spec_f_2 (normI 1 x_1) (normI 2 x_2) - \<epsilon>) \<le> f_ann (normI 1 x_1) (normI 2 x_2) \<and> f_ann (normI 1 x_1) (normI 2 x_2) \<le> normO 1 (norm_spec_f_2 (normI 1 x_1) (normI 2 x_2) + \<epsilon>)\<close> \<open>normO 1 (P * denormI 1 (normI 1 x_1) + D * denormI 2 (normI 2 x_2) - \<epsilon>) \<le> f_ann (normI 1 x_1) (normI 2 x_2) \<and> f_ann (normI 1 x_1) (normI 2 x_2) \<le> normO 1 (P * denormI 1 (normI 1 x_1) + D * denormI 2 (normI 2 x_2) + \<epsilon>) \<longrightarrow> denormO 1 (normO 1 (P * denormI 1 (normI 1 x_1) + D * denormI 2 (normI 2 x_2) - \<epsilon>)) \<le> denormO 1 (f_ann (normI 1 x_1) (normI 2 x_2)) \<and> denormO 1 (f_ann (normI 1 x_1) (normI 2 x_2)) \<le> denormO 1 (normO 1 (P * denormI 1 (normI 1 x_1) + D * denormI 2 (normI 2 x_2) + \<epsilon>))\<close> \<open>normO 1 (norm_spec_f_2 (normI 1 x_1) (normI 2 x_2) - \<epsilon>) \<le> f_ann (normI 1 x_1) (normI 2 x_2) \<and> f_ann (normI 1 x_1) (normI 2 x_2) \<le> normO 1 (norm_spec_f_2 (normI 1 x_1) (normI 2 x_2) + \<epsilon>) \<longrightarrow> normO 1 (P * denormI 1 (normI 1 x_1) + D * denormI 2 (normI 2 x_2) - \<epsilon>) \<le> f_ann (normI 1 x_1) (normI 2 x_2) \<and> f_ann (normI 1 x_1) (normI 2 x_2) \<le> normO 1 (P * denormI 1 (normI 1 x_1) + D * denormI 2 (normI 2 x_2) + \<epsilon>)\<close> m3 by argo
-
-    from 1 have goal3:"normI 1 x_1 \<ge> normI 1 (inRanges(1).1) \<and> 
+    from assms have goal3:"normI 1 x_1 \<ge> normI 1 (inRanges(1).1) \<and> 
           normI 1 x_1 \<le> normI 1 (inRanges(1).2) \<and>
           normI 2 x_2 \<ge> normI 2 (inRanges(2).1) \<and>
           normI 2 x_2 \<le> normI 2 (inRanges(2).2)"
       by (smt (verit) assms(2) mono_normI)
 
+    have "y_1 = P * x_1 + D * x_2 \<longrightarrow> \<bar>denormO 1 (f_ann (normI 1 x_1) (normI 2 x_2)) - y_1\<bar> \<le> \<epsilon>"
+      by (metis \<open>(P * denormI 1 (normI 1 x_1) + D * denormI 2 (normI 2 x_2) - \<epsilon> \<le> denormO 1 (f_ann (normI 1 x_1) (normI 2 x_2)) \<and> denormO 1 (f_ann (normI 1 x_1) (normI 2 x_2)) \<le> P * denormI 1 (normI 1 x_1) + D * denormI 2 (normI 2 x_2) + \<epsilon>) = (P * x_1 + D * x_2 - \<epsilon> \<le> denormO 1 (f_ann (normI 1 x_1) (normI 2 x_2)) \<and> denormO 1 (f_ann (normI 1 x_1) (normI 2 x_2)) \<le> P * x_1 + D * x_2 + \<epsilon>)\<close> \<open>(P * x_1 + D * x_2 - \<epsilon> \<le> denormO 1 (f_ann (normI 1 x_1) (normI 2 x_2)) \<and> denormO 1 (f_ann (normI 1 x_1) (normI 2 x_2)) \<le> P * x_1 + D * x_2 + \<epsilon>) = (\<bar>denormO 1 (f_ann (normI 1 x_1) (normI 2 x_2)) - (P * x_1 + D * x_2)\<bar> \<le> \<epsilon>)\<close> \<open>(denormO 1 (normO 1 (P * denormI 1 (normI 1 x_1) + D * denormI 2 (normI 2 x_2) - \<epsilon>)) \<le> denormO 1 (f_ann (normI 1 x_1) (normI 2 x_2)) \<and> denormO 1 (f_ann (normI 1 x_1) (normI 2 x_2)) \<le> denormO 1 (normO 1 (P * denormI 1 (normI 1 x_1) + D * denormI 2 (normI 2 x_2) + \<epsilon>))) = (P * denormI 1 (normI 1 x_1) + D * denormI 2 (normI 2 x_2) - \<epsilon> \<le> denormO 1 (f_ann (normI 1 x_1) (normI 2 x_2)) \<and> denormO 1 (f_ann (normI 1 x_1) (normI 2 x_2)) \<le> P * denormI 1 (normI 1 x_1) + D * denormI 2 (normI 2 x_2) + \<epsilon>)\<close> \<open>(normO 1 (P * denormI 1 (normI 1 x_1) + D * denormI 2 (normI 2 x_2) - \<epsilon>) \<le> f_ann (normI 1 x_1) (normI 2 x_2) \<and> f_ann (normI 1 x_1) (normI 2 x_2) \<le> normO 1 (P * denormI 1 (normI 1 x_1) + D * denormI 2 (normI 2 x_2) + \<epsilon>)) = (denormO 1 (normO 1 (P * denormI 1 (normI 1 x_1) + D * denormI 2 (normI 2 x_2) - \<epsilon>)) \<le> denormO 1 (f_ann (normI 1 x_1) (normI 2 x_2)) \<and> denormO 1 (f_ann (normI 1 x_1) (normI 2 x_2)) \<le> denormO 1 (normO 1 (P * denormI 1 (normI 1 x_1) + D * denormI 2 (normI 2 x_2) + \<epsilon>)))\<close> \<open>normI 1 (fst (inRanges(1)\<^sub>s)) \<le> normI 1 x_1 \<and> normI 1 x_1 \<le> normI 1 (snd (inRanges(1)\<^sub>s)) \<and> normI 2 (fst (inRanges(2)\<^sub>s)) \<le> normI 2 x_2 \<and> normI 2 x_2 \<le> normI 2 (snd (inRanges(2)\<^sub>s)) \<and> normO 1 (norm_spec (snd (thm2_TEMP.int(1)\<^sub>s)) (snd (thm2_TEMP.int(2)\<^sub>s)) - \<epsilon>) \<le> f_ann (normI 1 x_1) (normI 2 x_2) \<and> f_ann (normI 1 x_1) (normI 2 x_2) \<le> normO 1 (norm_spec (fst (thm2_TEMP.int(1)\<^sub>s)) (fst (thm2_TEMP.int(2)\<^sub>s)) + \<epsilon>) \<longrightarrow> normO 1 (norm_spec (normI 1 x_1) (normI 2 x_2) - \<epsilon>) \<le> f_ann (normI 1 x_1) (normI 2 x_2) \<and> f_ann (normI 1 x_1) (normI 2 x_2) \<le> normO 1 (norm_spec (normI 1 x_1) (normI 2 x_2) + \<epsilon>)\<close> goal3 linorder_linear m3 norm_spec_def)
 
-    show "y_1 = P * x_1 + D * x_2 \<longrightarrow> \<bar>denormO 1 (f_ann (normI 1 x_1) (normI 2 x_2)) - y_1\<bar> \<le> \<epsilon>"
-      using goal2 goal3 by fastforce
-
+    thus "?thesis" 
+      using assms(1) conf_vcs by (auto)
 
   qed
 
